1) simplified subblock-opsem: removed invariant variables from states; big-step opsem doesn't need to take the whole stack as a state, the current frame is sufficient. llvm-opsem can be simplified too.
2) defined TV for blocks and functions, proved correctness within a
block. 

We need one more property of SE: weakening or strengthening
symbolic mapping with unused variables (that are not used or defined by
SE) does not change results, and this should also be true for the denotation of
SE. The opsem of each function does not know how many local
variables are defined within this function, which updates or adds
defined variables at runtime. So when defining TV for functions, we
don't know which variables SE are using for each subblock (We need to
let SE match opsem that works on only used/defined variables). We can take
all variable in this function for inputs of SE, and then weaken or strenthen them at each
subblock to prove the its result denotes opsem. We can also extend the syntax and opsem to get the list of local
variables with undefined values at the beginning of a function, then SE
doesn't need to hold the above property.



git-svn-id: https://webdav.seas.upenn.edu/svn/sol/vol@2534 eef5ea85-cc2e-0410-bd84-0fae1f012da8

src/TV/symexe_def.v
@@ -88,22 +88,13 @@ Inductive wf_cmds : list cmd -> Prop :=
 (* deterministic big-step for this new syntax with subblocks. *)
 
 Record ExecutionContext : Set := mkEC {
-CurFunction : fdef;
 CurBB       : block;
-CurCmds     : list subblock;         (* subblock to run within CurBB *)
-Terminator  : terminator;
 Locals      : GVMap;                 (* LLVM values used in this invocation *)
-Args        : list GenericValue;      
 Allocas     : list mblock            (* Track memory allocated by alloca *)
 }.
 
-Definition ECStack := list ExecutionContext.
-
 Record State : Set := mkState {
-CurSystem      : system;
-CurTatgetData  : layouts;
-CurProducts    : list product;
-ECS            : ECStack;
+Frame          : ExecutionContext;
 Globals        : GVMap;
 Mem            : mem
 }.
@@ -113,145 +104,178 @@ Variable switchToNewBasicBlock : block -> block -> GVMap -> GVMap.
 Variable lookupFdefViaIDFromSystem : system -> id -> option fdef.
 Variable getEntryBlock : fdef -> option block.
 
-Inductive dbCmd : State -> State -> trace -> Prop :=
-| dbBop: forall S TD Ps F B lc gl lc' gl' arg id bop sz v1 v2 gv3 EC cs c sbs tmn Mem als,
+Inductive dbCmd : layouts -> 
+                  GVMap -> list mblock -> GVMap -> mem -> 
+                  cmd -> 
+                  GVMap -> list mblock -> GVMap -> mem -> 
+                  trace -> Prop :=
+| dbBop: forall TD lc gl lc' gl' id bop sz v1 v2 gv3 Mem als,
   BOP TD lc gl bop sz v1 v2 = Some gv3 ->
   updateEnv lc gl id gv3 = (lc', gl') -> 
-  dbCmd 
-    (mkState S TD Ps ((mkEC F B ((subblock_intro ((insn_bop id bop sz v1 v2)::cs) c)::sbs) tmn lc arg als)::EC) gl Mem) 
-    (mkState S TD Ps ((mkEC F B ((subblock_intro cs c)::sbs) tmn lc' arg als)::EC) gl' Mem)
+  dbCmd TD
+    lc als gl Mem
+    (insn_bop id bop sz v1 v2)
+    lc' als gl' Mem
     trace_nil 
-| dbExtractValue : forall S TD Ps F B lc gl lc' gl' arg id t v gv gv' idxs EC cs c sbs tmn Mem als,
+| dbExtractValue : forall TD lc gl lc' gl' id t v gv gv' Mem als idxs,
   getOperandValue TD v lc gl = Some gv ->
   extractGenericValue TD t gv idxs = Some gv' ->
   updateEnv lc gl id gv' = (lc', gl') -> 
-  dbCmd 
-    (mkState S TD Ps ((mkEC F B ((subblock_intro ((insn_extractvalue id t v idxs)::cs) c)::sbs) tmn lc arg als)::EC) gl Mem) 
-    (mkState S TD Ps ((mkEC F B ((subblock_intro cs c)::sbs) tmn lc' arg als)::EC) gl' Mem)
+  dbCmd TD 
+    lc als gl Mem
+    (insn_extractvalue id t v idxs)
+    lc' als gl' Mem
     trace_nil 
-| dbInsertValue : forall S TD Ps F B lc gl lc' gl' arg id t v t' v' gv gv' gv'' idxs EC cs c sbs tmn Mem als,
+| dbInsertValue : forall TD lc gl lc' gl' id t v t' v' gv gv' gv'' idxs Mem als,
   getOperandValue TD v lc gl = Some gv ->
   getOperandValue TD v' lc gl = Some gv' ->
   insertGenericValue TD t gv idxs t' gv' = Some gv'' ->
   updateEnv lc gl id gv'' = (lc', gl') -> 
-  dbCmd 
-    (mkState S TD Ps ((mkEC F B ((subblock_intro ((insn_insertvalue id t v t' v' idxs)::cs) c)::sbs) tmn lc arg als)::EC) gl Mem) 
-    (mkState S TD Ps ((mkEC F B ((subblock_intro cs c)::sbs) tmn lc' arg als)::EC) gl' Mem)
+  dbCmd TD 
+    lc als gl Mem
+    (insn_insertvalue id t v t' v' idxs)
+    lc' als gl' Mem
     trace_nil 
-| dbMalloc : forall S TD Ps F B lc gl lc' gl' arg id t sz align EC cs c sbs tmn Mem als Mem' tsz mb,
+| dbMalloc : forall TD lc gl lc' gl' id t sz align Mem als Mem' tsz mb,
   getTypeAllocSize TD t = Some tsz ->
   malloc TD Mem (tsz * sz) align = Some (Mem', mb) ->
   updateEnv lc gl id (ptr2GV TD (mb, 0)) = (lc', gl') -> 
-  dbCmd 
-    (mkState S TD Ps ((mkEC F B ((subblock_intro ((insn_malloc id t sz align)::cs) c)::sbs) tmn lc arg als)::EC) gl Mem) 
-    (mkState S TD Ps ((mkEC F B ((subblock_intro cs c)::sbs) tmn lc' arg als)::EC) gl' Mem')
+  dbCmd TD 
+    lc als gl Mem
+    (insn_malloc id t sz align)
+    lc' als gl' Mem'
     trace_nil
-| dbFree : forall S TD Ps F B lc gl arg fid t v EC cs c sbs tmn Mem als Mem' mptr,
+| dbFree : forall TD lc gl fid t v Mem als Mem' mptr,
   getOperandPtr TD v lc gl = Some mptr ->
   free Mem mptr = Some Mem'->
-  dbCmd 
-    (mkState S TD Ps ((mkEC F B ((subblock_intro ((insn_free fid t v)::cs) c)::sbs) tmn lc arg als)::EC) gl Mem) 
-    (mkState S TD Ps ((mkEC F B ((subblock_intro cs c)::sbs) tmn lc arg als)::EC) gl Mem')
+  dbCmd TD 
+    lc als gl Mem
+    (insn_free fid t v)
+    lc als gl Mem'
     trace_nil
-| dbAlloca : forall S TD Ps F B lc gl lc' gl' arg id t sz align EC cs c sbs tmn Mem als Mem' tsz mb,
+| dbAlloca : forall TD lc gl lc' gl' id t sz align Mem als Mem' tsz mb,
   getTypeAllocSize TD t = Some tsz ->
   malloc TD Mem (tsz * sz) align = Some (Mem', mb) ->
   updateEnv lc gl id (ptr2GV TD (mb, 0)) = (lc', gl') -> 
-  dbCmd 
-    (mkState S TD Ps ((mkEC F B ((subblock_intro ((insn_alloca id t sz align)::cs) c)::sbs) tmn lc arg als)::EC) gl Mem) 
-    (mkState S TD Ps ((mkEC F B ((subblock_intro cs c)::sbs) tmn lc' arg (mb::als))::EC) gl' Mem')
+  dbCmd TD 
+    lc als gl Mem
+    (insn_alloca id t sz align)
+    lc' (mb::als) gl' Mem'
     trace_nil
-| dbLoad : forall S TD Ps F B lc gl lc' gl' arg id t v EC cs c sbs tmn Mem als mp gv,
+| dbLoad : forall TD lc gl lc' gl' id t v Mem als mp gv,
   getOperandPtr TD v lc gl = Some mp ->
   mload TD Mem mp t = Some gv ->
   updateEnv lc gl id gv = (lc', gl') -> 
-  dbCmd 
-    (mkState S TD Ps ((mkEC F B ((subblock_intro ((insn_load id t v)::cs) c)::sbs) tmn lc arg als)::EC) gl Mem) 
-    (mkState S TD Ps ((mkEC F B ((subblock_intro cs c)::sbs) tmn lc' arg als)::EC) gl' Mem)
+  dbCmd TD 
+    lc als gl Mem
+    (insn_load id t v)
+    lc' als gl' Mem
     trace_nil
-| dbStore : forall S TD Ps F B lc gl arg sid t v1 v2 EC cs c sbs tmn Mem als mp2 gv1 Mem',
+| dbStore : forall TD lc gl sid t v1 v2 Mem als mp2 gv1 Mem',
   getOperandValue TD v1 lc gl = Some gv1 ->
   getOperandPtr TD v2 lc gl = Some mp2 ->
   mstore TD Mem mp2 t gv1 = Some Mem' ->
-  dbCmd 
-    (mkState S TD Ps ((mkEC F B ((subblock_intro ((insn_store sid t v1 v2)::cs) c)::sbs) tmn lc arg als)::EC) gl Mem) 
-    (mkState S TD Ps ((mkEC F B ((subblock_intro cs c)::sbs) tmn lc arg als)::EC) gl Mem')
+  dbCmd TD 
+    lc als gl Mem
+    (insn_store sid t v1 v2)
+    lc als gl Mem'
     trace_nil
-| dbGEP : forall S TD Ps F B lc gl lc' gl' arg id inbounds t v idxs EC mp mp' cs c sbs tmn Mem als,
+| dbGEP : forall TD lc gl lc' gl' id inbounds t v idxs mp mp' Mem als,
   getOperandPtr TD v lc gl = Some mp ->
   GEP TD lc gl t mp idxs inbounds = Some mp' ->
   updateEnv lc gl id (ptr2GV TD mp') = (lc', gl') -> 
-  dbCmd 
-    (mkState S TD Ps ((mkEC F B ((subblock_intro ((insn_gep id inbounds t v idxs)::cs) c)::sbs) tmn lc arg als)::EC) gl Mem) 
-    (mkState S TD Ps ((mkEC F B ((subblock_intro cs c)::sbs) tmn lc' arg als)::EC) gl' Mem)
+  dbCmd TD 
+    lc als gl Mem
+    (insn_gep id inbounds t v idxs)
+    lc' als gl' Mem
     trace_nil 
-| dbExt : forall S TD Ps F B lc gl arg id extop t1 v1 t2 gv2 EC cs c sbs tmn lc' gl' Mem als,
+| dbExt : forall TD lc gl id extop t1 v1 t2 gv2 lc' gl' Mem als,
   EXT TD lc gl extop t1 v1 t2 = Some gv2 ->
   updateEnv lc gl id gv2 = (lc', gl') -> 
-  dbCmd 
-    (mkState S TD Ps ((mkEC F B ((subblock_intro ((insn_ext id extop t1 v1 t2)::cs) c)::sbs) tmn lc arg als)::EC) gl Mem) 
-    (mkState S TD Ps ((mkEC F B ((subblock_intro cs c)::sbs) tmn lc' arg als)::EC) gl' Mem)
+  dbCmd TD 
+    lc als gl Mem
+    (insn_ext id extop t1 v1 t2)
+    lc' als gl' Mem
     trace_nil
-| dbCast : forall S TD Ps F B lc gl arg id castop t1 v1 t2 gv2 EC cs c sbs tmn lc' gl' Mem als,
+| dbCast : forall TD lc gl id castop t1 v1 t2 gv2 lc' gl' Mem als,
   CAST TD lc gl castop t1 v1 t2 = Some gv2 ->
   updateEnv lc gl id gv2 = (lc', gl') -> 
-  dbCmd 
-    (mkState S TD Ps ((mkEC F B ((subblock_intro ((insn_cast id castop t1 v1 t2)::cs) c)::sbs) tmn lc arg als)::EC) gl Mem) 
-    (mkState S TD Ps ((mkEC F B ((subblock_intro cs c)::sbs) tmn lc' arg als)::EC) gl' Mem)
+  dbCmd TD 
+    lc als gl Mem
+    (insn_cast id castop t1 v1 t2)
+    lc' als gl' Mem
     trace_nil
-| dbIcmp : forall S TD Ps F B lc gl arg id cond t v1 v2 gv3 EC cs c sbs tmn lc' gl' Mem als,
+| dbIcmp : forall TD lc gl id cond t v1 v2 gv3 lc' gl' Mem als,
   ICMP TD lc gl cond t v1 v2 = Some gv3 ->
   updateEnv lc gl id gv3 = (lc', gl') -> 
-  dbCmd 
-    (mkState S TD Ps ((mkEC F B ((subblock_intro ((insn_icmp id cond t v1 v2)::cs) c)::sbs) tmn lc arg als)::EC) gl Mem) 
-    (mkState S TD Ps ((mkEC F B ((subblock_intro cs c)::sbs) tmn lc' arg als)::EC) gl' Mem)
+  dbCmd TD 
+    lc als gl Mem
+    (insn_icmp id cond t v1 v2)
+    lc' als gl' Mem
     trace_nil
-| dbSelect : forall S TD Ps F B lc gl arg id v0 t v1 v2 cond EC cs c sbs tmn lc' gl' Mem als gv1 gv2,
+| dbSelect : forall TD lc gl id v0 t v1 v2 cond lc' gl' Mem als gv1 gv2,
   getOperandInt TD 1 v0 lc gl = Some cond ->
   getOperandValue TD v1 lc gl = Some gv1 ->
   getOperandValue TD v2 lc gl = Some gv2 ->
   (lc', gl') = (if cond
                then updateEnv lc gl id gv1
                else updateEnv lc gl id gv2) ->
-  dbCmd 
-    (mkState S TD Ps ((mkEC F B ((subblock_intro ((insn_select id v0 t v1 v2)::cs) c)::sbs) tmn lc arg als)::EC) gl Mem) 
-    (mkState S TD Ps ((mkEC F B ((subblock_intro cs c)::sbs) tmn lc' arg als)::EC) gl' Mem)
+  dbCmd TD 
+    lc als gl Mem
+    (insn_select id v0 t v1 v2)
+    lc' als gl' Mem
     trace_nil
 .
 
-Inductive dbTerminator : State -> State -> trace -> Prop :=
-| dbBranch : forall S TD Ps F B lc gl arg bid Cond l1 l2 c
-                              l' ps' sbs' tmn' lc' EC Mem als,   
+Inductive dbTerminator : 
+  system -> layouts -> 
+  block -> GVMap -> GVMap -> 
+  terminator -> 
+  block -> GVMap -> 
+  trace -> Prop :=
+| dbBranch : forall S TD B lc gl bid Cond l1 l2 c
+                              l' ps' sbs' tmn' lc',   
   getOperandInt TD 1 Cond lc gl = Some c ->
   Some (block_intro l' ps' sbs' tmn') = (if c 
                then lookupBlockViaLabelFromSystem S l1
                else lookupBlockViaLabelFromSystem S l2) ->
   lc' = switchToNewBasicBlock (block_intro l' ps' sbs' tmn') B lc ->
-  dbTerminator 
-    (mkState S TD Ps ((mkEC F B nil (insn_br bid Cond l1 l2) lc arg als)::EC) gl Mem)
-    (mkState S TD Ps ((mkEC F (block_intro l' ps' sbs' tmn') sbs' tmn' lc' arg als)::EC) gl Mem)
+  dbTerminator S TD 
+    B lc gl
+    (insn_br bid Cond l1 l2)
+    (block_intro l' ps' sbs' tmn') lc' 
     trace_nil 
-| dbBranch_uncond : forall S TD Ps F B lc gl arg l bid
-                              l' ps' sbs' tmn' lc' EC Mem als,   
+| dbBranch_uncond : forall S TD B lc gl l bid
+                              l' ps' sbs' tmn' lc',   
   Some (block_intro l' ps' sbs' tmn') = (lookupBlockViaLabelFromSystem S l) ->
   lc' = switchToNewBasicBlock (block_intro l' ps' sbs' tmn') B lc ->
-  dbTerminator 
-    (mkState S TD Ps ((mkEC F B nil (insn_br_uncond bid l) lc arg als)::EC) gl Mem)
-    (mkState S TD Ps ((mkEC F (block_intro l' ps' sbs' tmn') sbs' tmn' lc' arg als)::EC) gl Mem)
+  dbTerminator S TD
+    B lc gl
+    (insn_br_uncond bid l) 
+    (block_intro l' ps' sbs' tmn') lc'
     trace_nil 
 .
 
-Inductive dbCmds : State -> State -> trace -> Prop :=
-| dbCmds_nil : forall S, dbCmds S S trace_nil
-| dbCmds_cons : forall S1 S2 S3 t1 t2,
-    dbCmd S1 S2 t1 ->
-    dbCmds S2 S3 t2 ->
-    dbCmds S1 S3 (trace_app t1 t2).
+Inductive dbCmds : layouts -> 
+                   GVMap -> list mblock -> GVMap -> mem -> 
+                   list cmd -> 
+                   GVMap -> list mblock -> GVMap -> mem -> 
+                   trace -> Prop :=
+| dbCmds_nil : forall TD lc als gl Mem, dbCmds TD lc als gl Mem nil lc als gl Mem trace_nil
+| dbCmds_cons : forall TD c cs lc1 als1 gl1 Mem1 t1 t2 lc2 als2 gl2 Mem2
+                       lc3 als3 gl3 Mem3,
+    dbCmd TD lc1 als1 gl1 Mem1 c lc2 als2 gl2 Mem2 t1 ->
+    dbCmds TD lc2 als2 gl2 Mem2 cs lc3 als3 gl3 Mem3 t2 ->
+    dbCmds TD lc1 als1 gl1 Mem1 (c::cs) lc3 als3 gl3 Mem3 (trace_app t1 t2).
 
-Inductive dbCall : State -> State -> trace -> Prop :=
-| dbCall_intro : forall S TD Ps F B lc gl arg rid noret tailc rt fid lp gl' gl'' sbs tmn
-                       EC Rid oResult tr lc'' B' lc' Mem Mem' als' als Mem'',
-  dbFdef fid rt lp S TD Ps ((mkEC F B ((subblock_intro nil (insn_call rid noret tailc rt fid lp))::sbs) tmn lc arg als)::EC) lc gl Mem lc' gl' als' Mem' B' Rid oResult tr ->
+Inductive dbCall : system -> layouts -> list product -> 
+                   GVMap -> GVMap -> mem -> 
+                   call -> 
+                   GVMap -> GVMap -> mem -> 
+                   trace -> Prop :=
+| dbCall_intro : forall S TD Ps lc gl rid noret tailc rt fid lp gl' gl''
+                       Rid oResult tr lc'' lc' Mem Mem' als' Mem'',
+  dbFdef fid rt lp S TD Ps lc gl Mem lc' gl' als' Mem' Rid oResult tr ->
   (lc'', gl'') = 
     match noret with
     | false =>
@@ -269,59 +293,90 @@ Inductive dbCall : State -> State -> trace -> Prop :=
     | true => (lc, gl')
     end ->
   free_allocas Mem' als' = Some Mem'' ->
-  dbCall 
-    (mkState S TD Ps ((mkEC F B ((subblock_intro nil (insn_call rid noret tailc rt fid lp))::sbs) tmn lc arg als)::EC) gl Mem) 
-    (mkState S TD Ps ((mkEC F B sbs tmn lc'' arg als)::EC) gl'' Mem'') 
+  dbCall S TD Ps 
+    lc gl Mem
+    (insn_call rid noret tailc rt fid lp)
+    lc'' gl'' Mem'' 
     tr
-with dbSubblock : State -> State -> trace -> Prop :=
-| dbSubblock_intro : forall state1 state2 tr1 state3 tr2,
-  dbCmds state1 state2 tr1 ->
-  dbCall state2 state3 tr2 ->
-  dbSubblock state1 state3 (trace_app tr1 tr2)
-with dbSubblocks : State -> State -> trace -> Prop :=
-| dbSubblocks_nil : forall S, dbSubblocks S S trace_nil
-| dbSubblocks_cond : forall S1 S2 S3 t1 t2,
-    dbSubblock S1 S2 t1 ->
-    dbSubblocks S2 S3 t2 ->
-    dbSubblocks S1 S3 (trace_app t1 t2)
-with dbBlock : State -> State -> trace -> Prop :=
-| dbBlock_intro : forall state1 state2 tr1 state3 tr2,
-  dbSubblocks state1 state2 tr1 ->
-  dbTerminator state2 state3 tr2 ->
-  dbBlock state1 state3 (trace_app tr1 tr2)
-with dbBlocks : State -> State -> trace -> Prop :=
-| dbBlocks_nil : forall S, dbBlocks S S trace_nil
-| dbBlocks_cons : forall S1 S2 S3 t1 t2,
-    dbBlock S1 S2 t1 ->
-    dbBlocks S2 S3 t2 ->
-    dbBlocks S1 S3 (trace_app t1 t2)
-with dbFdef : id -> typ -> list_param -> system -> layouts -> list product -> list ExecutionContext -> GVMap -> GVMap -> mem -> GVMap -> GVMap -> list mblock -> mem -> block -> id -> option value -> trace -> Prop :=
+with dbSubblock : system -> layouts -> list product -> 
+                  GVMap -> list mblock -> GVMap -> mem -> 
+                  subblock -> 
+                  GVMap -> list mblock -> GVMap -> mem -> 
+                  trace -> Prop :=
+| dbSubblock_intro : forall S TD Ps lc1 als1 gl1 Mem1 cs call0 lc2 als2 gl2 Mem2 tr1 
+                     lc3 gl3 Mem3 tr2,
+  dbCmds TD lc1 als1 gl1 Mem1 cs lc2 als2 gl2 Mem2 tr1 ->
+  dbCall S TD Ps lc2 gl2 Mem2 call0 lc3 gl3 Mem3 tr2 ->
+  dbSubblock S TD Ps 
+             lc1 als1 gl1 Mem1
+             (subblock_intro cs call0) 
+             lc3 als2 gl3 Mem3
+             (trace_app tr1 tr2)
+with dbSubblocks : system -> layouts -> list product -> 
+                   GVMap -> list mblock -> GVMap -> mem -> 
+                   list subblock -> 
+                   GVMap -> list mblock -> GVMap -> mem -> 
+                   trace -> Prop :=
+| dbSubblocks_nil : forall S TD Ps lc als gl Mem, 
+    dbSubblocks S TD Ps lc als gl Mem nil lc als gl Mem trace_nil
+| dbSubblocks_cond : forall S TD Ps lc1 als1 gl1 Mem1 lc2 als2 gl2 Mem2 lc3 als3 gl3 Mem3 sb sbs t1 t2,
+    dbSubblock S TD Ps lc1 als1 gl1 Mem1 sb lc2 als2 gl2 Mem2 t1 ->
+    dbSubblocks S TD Ps lc2 als2 gl2 Mem2 sbs lc3 als3 gl3 Mem3 t2 ->
+    dbSubblocks S TD Ps lc1 als1 gl1 Mem1 (sb::sbs) lc3 als3 gl3 Mem3 (trace_app t1 t2)
+with dbBlock : system -> layouts -> list product -> list GenericValue -> State -> State -> trace -> Prop :=
+| dbBlock_intro : forall S TD Ps tr1 tr2 l ps sbs tmn lc1 als1 gl1 Mem1
+                         lc2 als2 gl2 Mem2 lc3 B' arg,
+  dbSubblocks S TD Ps
+    lc1 als1 gl1 Mem1
+    sbs
+    lc2 als2 gl2 Mem2
+    tr1 ->
+  dbTerminator S TD
+    (block_intro l ps sbs tmn) lc2 gl2
+    tmn
+    B' lc3
+    tr2 ->
+  dbBlock S TD Ps arg
+    (mkState (mkEC (block_intro l ps sbs tmn) lc1 als1) gl1 Mem1)
+    (mkState (mkEC B' lc3 als2) gl2 Mem2)
+    (trace_app tr1 tr2)
+with dbBlocks : system -> layouts -> list product -> list GenericValue -> State -> State -> trace -> Prop :=
+| dbBlocks_nil : forall S TD Ps arg state, dbBlocks S TD Ps arg state state trace_nil
+| dbBlocks_cons : forall S TD Ps arg S1 S2 S3 t1 t2,
+    dbBlock S TD Ps arg S1 S2 t1 ->
+    dbBlocks S TD Ps arg S2 S3 t2 ->
+    dbBlocks S TD Ps arg S1 S3 (trace_app t1 t2)
+with dbFdef : id -> typ -> list_param -> system -> layouts -> list product -> GVMap -> GVMap -> mem -> GVMap -> GVMap -> list mblock -> mem -> id -> option value -> trace -> Prop :=
 | dbFdef_func : forall S TD Ps gl fid lp lc rid
-                            l' ps' cs' tmn' rt la lb B'' Result lc' gl' tr ECs Mem Mem' als',
+                       l1 ps1 sbs1 tmn1 rt la lb Result lc1 gl1 tr1 Mem Mem1 als1
+                       l2 ps2 sbs2 lc2 als2 gl2 Mem2 tr2,
   lookupFdefViaIDFromSystem S fid = Some (fdef_intro (fheader_intro rt fid la) lb) ->
-  getEntryBlock (fdef_intro (fheader_intro rt fid la) lb) = Some (block_intro l' ps' cs' tmn') ->
-  dbBlocks 
-    (mkState S TD Ps ((mkEC (fdef_intro (fheader_intro rt fid la) lb) 
-                             (block_intro l' ps' cs' tmn') cs' tmn' (initLocals la (params2GVs TD lp lc gl))
-                            (params2GVs TD lp lc gl) nil)::ECs) gl Mem)
-    (mkState S TD Ps ((mkEC (fdef_intro (fheader_intro rt fid la) lb) 
-                             B'' nil (insn_return rid rt Result) lc'
-                            (params2GVs TD lp lc gl) als')::ECs) gl' Mem')
-    tr ->
-  dbFdef fid rt lp S TD Ps ECs lc gl Mem lc' gl' als' Mem' B'' rid (Some Result) tr
+  getEntryBlock (fdef_intro (fheader_intro rt fid la) lb) = Some (block_intro l1 ps1 sbs1 tmn1) ->
+  dbBlocks S TD Ps (params2GVs TD lp lc gl)
+    (mkState (mkEC (block_intro l1 ps1 sbs1 tmn1) (initLocals la (params2GVs TD lp lc gl)) nil) gl Mem)
+    (mkState (mkEC (block_intro l2 ps2 sbs2 (insn_return rid rt Result)) lc1 als1) gl1 Mem1)
+    tr1 ->
+  dbSubblocks S TD Ps 
+    lc1 als1 gl1 Mem1
+    sbs2
+    lc2 als2 gl2 Mem2
+    tr2 ->
+  dbFdef fid rt lp S TD Ps lc gl Mem lc2 gl2 als2 Mem2 rid (Some Result) (trace_app tr1 tr2)
 | dbFdef_proc : forall S TD Ps gl fid lp lc rid
-                            l' ps' cs' tmn' rt la lb B'' lc' gl' tr ECs Mem Mem' als',
+                       l1 ps1 sbs1 tmn1 rt la lb lc1 gl1 tr1 Mem Mem1 als1
+                       l2 ps2 sbs2 lc2 als2 gl2 Mem2 tr2,
   lookupFdefViaIDFromSystem S fid = Some (fdef_intro (fheader_intro rt fid la) lb) ->
-  getEntryBlock (fdef_intro (fheader_intro rt fid la) lb) = Some (block_intro l' ps' cs' tmn') ->
-  dbBlocks 
-    (mkState S TD Ps ((mkEC (fdef_intro (fheader_intro rt fid la) lb) 
-                             (block_intro l' ps' cs' tmn') cs' tmn' (initLocals la (params2GVs TD lp lc gl))
-                            (params2GVs TD lp lc gl) nil)::ECs) gl Mem)
-    (mkState S TD Ps ((mkEC (fdef_intro (fheader_intro rt fid la) lb) 
-                             B'' nil (insn_return_void rid) lc'
-                            (params2GVs TD lp lc gl) als')::ECs) gl' Mem')
-    tr ->
-  dbFdef fid  rt lp S TD Ps ECs lc gl Mem lc' gl' als' Mem' B'' rid None tr
+  getEntryBlock (fdef_intro (fheader_intro rt fid la) lb) = Some (block_intro l1 ps1 sbs1 tmn1) ->
+  dbBlocks S TD Ps (params2GVs TD lp lc gl) 
+    (mkState (mkEC (block_intro l1 ps1 sbs1 tmn1) (initLocals la (params2GVs TD lp lc gl)) nil) gl Mem)
+    (mkState (mkEC (block_intro l2 ps2 sbs2 (insn_return_void rid)) lc2 als2) gl2 Mem2)
+    tr1 ->
+  dbSubblocks S TD Ps 
+    lc1 als1 gl1 Mem1
+    sbs2
+    lc2 als2 gl2 Mem2
+    tr2 ->
+  dbFdef fid  rt lp S TD Ps lc gl Mem lc2 gl2 als2 Mem2 rid None (trace_app tr1 tr2)
 .
 
 Scheme dbCall_ind2 := Induction for dbCall Sort Prop
@@ -360,49 +415,22 @@ Hint Constructors dbCmd dbCmds dbTerminator dbCall
                   dbSubblock dbSubblocks dbBlock dbBlocks dbFdef.
 
 (* properties of opsem *)
-Lemma dbCmd_inversion : forall a cs S TD Ps F B call0 sbs tmn arg als ECs lc gl Mem1 state2 tr,
-  dbCmd (mkState S TD Ps ((mkEC F B ((subblock_intro (a::cs) call0)::sbs) tmn lc arg als)::ECs) gl Mem1)
-        state2
-        tr ->
-  exists lc', exists gl', exists als', exists Mem2,
-    state2 = (mkState S TD Ps ((mkEC F B ((subblock_intro cs call0)::sbs) tmn lc' arg als')::ECs) gl' Mem2).
-Proof.
-  intros a cs S TD Ps F B call0 sbs tmn arg0 als ECs lc gl Mem1 state2 tr HdbCmd.
-  inversion HdbCmd; subst; 
-  try solve [
-    exists lc'; exists gl'; exists als; exists Mem1; auto |
-    exists lc'; exists gl'; exists als; exists Mem'; auto |
-    exists lc; exists gl; exists als; exists Mem'; auto |
-    exists lc'; exists gl'; exists (mb::als); exists Mem'; auto
-  ].
-Qed.
-
-Lemma dbCmd_eqEnv : forall S TD Ps F B c cs cs' call0 sbs tmn lc1 arg als1 ECs gl1 Mem1 lc2 als2 gl2 Mem2 tr lc2' gl2',
-  dbCmd (mkState S TD Ps ((mkEC F B ((subblock_intro (c::cs) call0)::sbs) tmn lc1 arg als1)::ECs) gl1 Mem1)
-        (mkState S TD Ps ((mkEC F B ((subblock_intro cs' call0)::sbs) tmn lc2 arg als2)::ECs) gl2 Mem2)
-        tr ->
+Lemma dbCmd_eqEnv : forall TD c lc1  als1 gl1 Mem1 lc2 als2 gl2 Mem2 tr lc2' gl2',
+  dbCmd TD lc1 als1 gl1 Mem1 c lc2 als2 gl2 Mem2 tr ->
   eqEnv lc2 gl2 lc2' gl2' ->
-  dbCmd (mkState S TD Ps ((mkEC F B ((subblock_intro (c::cs) call0)::sbs) tmn lc1 arg als1)::ECs) gl1 Mem1)
-        (mkState S TD Ps ((mkEC F B ((subblock_intro cs' call0)::sbs) tmn lc2' arg als2)::ECs) gl2' Mem2)
-        tr.
+  dbCmd TD lc1 als1 gl1 Mem1 c lc2' als2 gl2' Mem2 tr.
 Admitted.
 
-Lemma dbCmds_eqEnv : forall S TD Ps F B cs cs' call0 sbs tmn lc1 arg als1 ECs gl1 Mem1 lc2 als2 gl2 Mem2 tr lc2' gl2',
-  dbCmds (mkState S TD Ps ((mkEC F B ((subblock_intro cs call0)::sbs) tmn lc1 arg als1)::ECs) gl1 Mem1)
-        (mkState S TD Ps ((mkEC F B ((subblock_intro cs' call0)::sbs) tmn lc2 arg als2)::ECs) gl2 Mem2)
-        tr ->
+Lemma dbCmds_eqEnv : forall TD cs lc1 als1 gl1 Mem1 lc2 als2 gl2 Mem2 tr lc2' gl2',
+  dbCmds TD lc1 als1 gl1 Mem1 cs lc2 als2 gl2 Mem2 tr ->
   eqEnv lc2 gl2 lc2' gl2' ->
-  dbCmds (mkState S TD Ps ((mkEC F B ((subblock_intro cs call0)::sbs) tmn lc1 arg als1)::ECs) gl1 Mem1)
-        (mkState S TD Ps ((mkEC F B ((subblock_intro cs' call0)::sbs) tmn lc2' arg als2)::ECs) gl2' Mem2)
-        tr.
+  dbCmds TD lc1 als1 gl1 Mem1 cs lc2' als2 gl2' Mem2 tr.
 Admitted.
 
-Lemma dbCmds_uniq : forall S TD Ps F B cs cs' call0 sbs tmn lc1 arg als1 ECs gl1 Mem1 lc2 als2 gl2 Mem2 tr,
+Lemma dbCmds_uniq : forall TD cs lc1 als1 gl1 Mem1 lc2 als2 gl2 Mem2 tr,
   uniq gl1 ->
   uniq lc1 ->
-  dbCmds (mkState S TD Ps ((mkEC F B ((subblock_intro cs call0)::sbs) tmn lc1 arg als1)::ECs) gl1 Mem1)
-        (mkState S TD Ps ((mkEC F B ((subblock_intro cs' call0)::sbs) tmn lc2 arg als2)::ECs) gl2 Mem2)
-        tr ->
+  dbCmds TD lc1 als1 gl1 Mem1 cs lc2 als2 gl2 Mem2 tr ->
   uniq gl2 /\ uniq lc2.
 Admitted.
 
@@ -1566,5 +1594,64 @@ Proof.
     apply H2 in H; auto.
 Qed.
 
+
+(* Definions below have not been used yet. *)
+
+Fixpoint subst_tt (id0:id) (s0:sterm) (s:sterm) : sterm :=
+match s with
+| sterm_val (value_id id1) => if id0 == id1 then s0 else s
+| sterm_val (value_const c) => sterm_val (value_const c)
+| sterm_bop op sz s1 s2 => 
+    sterm_bop op sz (subst_tt id0 s0 s1) (subst_tt id0 s0 s2)
+| sterm_extractvalue t1 s1 cs => 
+    sterm_extractvalue t1 (subst_tt id0 s0 s1) cs
+| sterm_insertvalue t1 s1 t2 s2 cs => 
+    sterm_insertvalue t1 (subst_tt id0 s0 s1) t2 (subst_tt id0 s0 s2) cs
+| sterm_malloc m1 t1 sz align => 
+    sterm_malloc (subst_tm id0 s0 m1) t1 sz align
+| sterm_alloca m1 t1 sz align => 
+    sterm_alloca (subst_tm id0 s0 m1) t1 sz align
+| sterm_load m1 t1 s1 => 
+    sterm_load (subst_tm id0 s0 m1) t1 (subst_tt id0 s0 s1)
+| sterm_gep inbounds t1 s1 ls2 =>
+    sterm_gep inbounds t1 (subst_tt id0 s0 s1) (List.map (subst_tt id0 s0) ls2)
+| sterm_ext extop t1 s1 t2 => 
+    sterm_ext extop t1 (subst_tt id0 s0 s1) t2
+| sterm_cast castop t1 s1 t2 => 
+    sterm_cast castop t1 (subst_tt id0 s0 s1) t2
+| sterm_icmp cond t1 s1 s2 => 
+    sterm_icmp cond t1 (subst_tt id0 s0 s1) (subst_tt id0 s0 s2)
+| sterm_phi t1 lsl1 => 
+    sterm_phi t1 (List.map 
+                   (fun (sl1:sterm*l) => 
+                    let (s1,l1):=sl1 in 
+                    ((subst_tt id0 s0 s1), l1)
+                   ) 
+                   lsl1)
+| sterm_select s1 t1 s2 s3 => 
+    sterm_select (subst_tt id0 s0 s1) t1 (subst_tt id0 s0 s2) (subst_tt id0 s0 s3)
+end
+with subst_tm (id0:id) (s0:sterm) (m:smem) : smem :=
+match m with 
+| smem_init => smem_init
+| smem_malloc m1 t1 sz align => smem_malloc (subst_tm id0 s0 m1) t1 sz align
+| smem_free m1 t1 s1 => smem_free (subst_tm id0 s0 m1) t1 (subst_tt id0 s0 s1)
+| smem_alloca m1 t1 sz align => smem_alloca (subst_tm id0 s0 m1) t1 sz align
+| smem_load m1 t1 s1 => smem_load (subst_tm id0 s0 m1) t1 (subst_tt id0 s0 s1)
+| smem_store m1 t1 s1 s2 => smem_store (subst_tm id0 s0 m1) t1 (subst_tt id0 s0 s1) (subst_tt id0 s0 s2)
+end
+.
+
+Fixpoint subst_mt (sm:smap) (s:sterm) : sterm :=
+match sm with
+| nil => s
+| (id0, s0)::sm' => subst_mt sm' (subst_tt id0 s0 s)
+end.
+
+Fixpoint subst_mm (sm:smap) (m:smem) : smem :=
+match sm with
+| nil => m
+| (id0, s0)::sm' => subst_mm sm' (subst_tm id0 s0 m)
+end.
 
 End SimpleSE.
